test/tactic_test.ml
@@ -1794,3 +1794,190 @@ let%expect_test "cancellation rev" =
     ========================================
     ∀x. ∀y. plus y x = plus z x ==> y = z
     |}]
+
+let%expect_test "length Nil = Zero" =
+  let open Theorems.Nat in
+  let open Theorems.ListTheory in
+  let length_const = make_const "length" [ (a, nat_ty) ] |> Result.get_ok in
+  let nil_nat = type_inst [ (a, nat_ty) ] nil |> Result.get_ok in
+
+  let length_nil = App (length_const, nil_nat) in
+  let goal = Result.get_ok (safe_make_eq length_nil zero) in
+
+  let next_tactic = next_tactic_of_list [ simp_tac ~with_asms:false ] in
+  (match prove ([], goal) next_tactic with
+  | Complete thm ->
+      print_endline "Proof Complete!";
+      Printing.print_thm thm
+  | Incomplete (asms, g) ->
+      print_endline "Proof Incomplete";
+      List.iter Printing.print_term asms;
+      Printing.print_term g);
+
+  [%expect
+    {|
+    Proof Complete!
+    ========================================
+    length Nil = Zero
+    |}]
+
+let%expect_test "length (Cons Zero Nil) = Suc Zero" =
+  let open Theorems.Nat in
+  let open Theorems.ListTheory in
+  let _ = length_def |> Result.get_ok in
+
+  let length_const = make_const "length" [ (a, nat_ty) ] |> Result.get_ok in
+  let nil_nat = type_inst [ (a, nat_ty) ] nil |> Result.get_ok in
+  let cons_nat = type_inst [ (a, nat_ty) ] cons |> Result.get_ok in
+
+  (* Cons Zero Nil *)
+  let cons_zero_nil = App (App (cons_nat, zero), nil_nat) in
+  let length_cons = App (length_const, cons_zero_nil) in
+  let goal = Result.get_ok (safe_make_eq length_cons n1) in
+
+  let next_tactic =
+    next_tactic_of_list @@ wrap_all with_no_trace [ simp_tac ]
+  in
+  (match prove ([], goal) next_tactic with
+  | Complete thm ->
+      print_endline "Proof Complete!";
+      Printing.print_thm thm
+  | Incomplete (asms, g) ->
+      print_endline "Proof Incomplete";
+      List.iter Printing.print_term asms;
+      Printing.print_term g);
+
+  [%expect
+    {|
+    Proof Complete!
+    ========================================
+    length (Cons Zero Nil) = Suc Zero
+    |}]
+
+let%expect_test "length_cons" =
+  let open Theorems.Nat in
+  let open Theorems.ListTheory in
+  let _ = length_def |> Result.get_ok in
+
+  let length_const = make_const "length" [ (a, nat_ty) ] |> Result.get_ok in
+  let cons_nat = type_inst [ (a, nat_ty) ] cons |> Result.get_ok in
+
+  let x = make_var "x" nat_ty in
+  let xs = make_var "xs" (TyCon ("list", [ nat_ty ])) in
+
+  (* length (Cons x xs) *)
+  let cons_x_xs = App (App (cons_nat, x), xs) in
+  let length_cons_x_xs = App (length_const, cons_x_xs) in
+
+  (* Suc (length xs) *)
+  let length_xs = App (length_const, xs) in
+  let suc_length_xs = App (suc, length_xs) in
+
+  (* ∀x. ∀xs. length (Cons x xs) = Suc (length xs) *)
+  let goal =
+    Derived.make_foralls [ x; xs ]
+      (Result.get_ok (safe_make_eq length_cons_x_xs suc_length_xs))
+  in
+
+  let next_tactic =
+    next_tactic_of_list @@ wrap_all with_no_trace [ gen_tac; gen_tac; simp_tac ]
+  in
+  (match prove ([], goal) next_tactic with
+  | Complete thm ->
+      print_endline "Proof Complete!";
+      Printing.print_thm thm
+  | Incomplete (asms, g) ->
+      print_endline "Proof Incomplete";
+      List.iter Printing.print_term asms;
+      Printing.print_term g);
+
+  [%expect
+    {|
+    Proof Complete!
+    ========================================
+    ∀x. ∀xs. length (Cons x xs) = Suc (length xs)
+    |}]
+
+(* xs = Nil ==> length xs = Zero *)
+let%expect_test "nil_implies_length_zero" =
+  let open Theorems.Nat in
+  let open Theorems.ListTheory in
+  let _ = length_def |> Result.get_ok in
+
+  let length_const = make_const "length" [ (a, nat_ty) ] |> Result.get_ok in
+  let nil_nat = type_inst [ (a, nat_ty) ] nil |> Result.get_ok in
+
+  let xs = make_var "xs" (TyCon ("list", [ nat_ty ])) in
+
+  (* xs = Nil *)
+  let xs_eq_nil = Result.get_ok (safe_make_eq xs nil_nat) in
+
+  (* length xs = Zero *)
+  let length_xs = App (length_const, xs) in
+  let length_eq_zero = Result.get_ok (safe_make_eq length_xs zero) in
+
+  (* ∀xs. xs = Nil ==> length xs = Zero *)
+  let goal = make_forall xs (make_imp xs_eq_nil length_eq_zero) in
+
+  let next_tactic =
+    next_tactic_of_list
+    @@ wrap_all with_no_trace
+         [
+           gen_tac; intro_tac; rewrite_tac |> with_assumption_rewrites; simp_tac;
+         ]
+  in
+  (match prove ([], goal) next_tactic with
+  | Complete thm ->
+      print_endline "Proof Complete!";
+      Printing.print_thm thm
+  | Incomplete (asms, g) ->
+      print_endline "Proof Incomplete";
+      List.iter Printing.print_term asms;
+      Printing.print_term g);
+
+  [%expect
+    {|
+    Proof Complete!
+    ========================================
+    ∀xs. xs = Nil ==> length xs = Zero
+    |}]
+
+(* length xs = Zero ==> xs = Nil *)
+let%expect_test "length_zero_implies_nil" =
+  let open Theorems.Nat in
+  let open Theorems.ListTheory in
+  let _ = length_def |> Result.get_ok in
+
+  let length_const = make_const "length" [ (a, nat_ty) ] |> Result.get_ok in
+  let nil_nat = type_inst [ (a, nat_ty) ] nil |> Result.get_ok in
+
+  let xs = make_var "xs" (TyCon ("list", [ nat_ty ])) in
+
+  (* length xs = Zero *)
+  let length_xs = App (length_const, xs) in
+  let length_eq_zero = Result.get_ok (safe_make_eq length_xs zero) in
+
+  (* xs = Nil *)
+  let xs_eq_nil = Result.get_ok (safe_make_eq xs nil_nat) in
+
+  (* ∀xs. length xs = Zero ==> xs = Nil *)
+  let goal = make_forall xs (make_imp length_eq_zero xs_eq_nil) in
+
+  let next_tactic = next_tactic_of_list [ induct_tac ] in
+  (match prove ([], goal) next_tactic with
+  | Complete thm ->
+      print_endline "Proof Complete!";
+      Printing.print_thm thm
+  | Incomplete (asms, g) ->
+      print_endline "Proof Incomplete";
+      List.iter print_term asms;
+      Printing.print_term g);
+
+  [%expect {|
+    (TyCon ("fun", [(TyCon ("list", [(TyVar "a")])); (TyCon ("bool", []))]))
+    (TyCon ("fun",
+       [(TyCon ("list", [(TyCon ("nat", []))])); (TyCon ("bool", []))]))
+    TypesDontAgree
+    Proof Incomplete
+    ∀xs. length xs = Zero ==> xs = Nil
+    |}]
